---
title: "Homework 12"
author: "Christophe Hunt"
date: "April 22, 2017"
output:
  pdf_document:
    fig_caption: yes
    keep_tex: yes
    includes:
      in_header: header.tex
    number_sections: yes
    toc: yes
    toc_depth: 2
  html_document:
    toc: yes
    toc_depth: '2'
always_allow_html: yes
---

\newpage

# Page 529: problem 1

Verify that the given function pair is a solution to the first-order system. 

$x = -e^t$, $y = e^t$       
$\frac{dx}{dt} = -y$, $\frac{dy}{dt} = -x$      

$\frac{dx}{dt} = \frac{d}{dt}(-e^t) = e^t = y$ ; $\frac{dx}{dt} = -y$   

$\frac{dy}{dt} = \frac{d}{dt}(e^t) = -e^t = x$ ; $\frac{dy}{dt} = -x$   

# Page 529: problem 6

Find and classify the rest points of the given autonomous system. 

$\frac{dx}{dt} = -(y-1)$, $\frac{dy}{dt} = x-2$

The rest point of the system is a point in the phase plane for which $f(x,y) = 0 and g(x,y) = 0$, then both the derivatives $\frac{dx}{dt} = 0$ and $\frac{dy}{dt}= 0$. 

when $y = 1$, $\frac{dx}{dt} = -(1-1)$; $\frac{dx}{dt}= 0$    
when $x = 2$, $\frac{dy}{dt} = 2 - 2$; $\frac{dy}{dt} = 0$   

$(2,1)$ is the rest point of the autonomous system $\frac{dx}{dt} = -(y-1)$, $\frac{dy}{dt} = x-2$   

# Page 546: problem 1

Apply the first and second derivative tests to the function 
$f(y) = y^a/e^{by}$ to show that $f(y) = y^a/e^{by}$ is a unique critical point that yields the relative maximum $f(a/b)$. Show also that $f(y)$ approaches zero as y tends to infinity. 

first derivative test 

$\frac{d(\frac{y^a}{e^{by}})}{dy} = 0$      
$\frac{e^{by}ay^{a-1}-y^abe^{by}}{e^{2by}}=0$      


$e^{by}ay^{a-1}(a-yb) = 0$
Since $e^{by}$ cannot be zero :
$y = \frac{a}{b}~or~y =0$

Second derivative test 

$\frac{d^2f(y)}{dy^2} = \frac{d\frac{ay^{a-1}-y^ab}{e^{by}}}{dy}$    
$\frac{d^2f(y)}{dy^2} = \frac{e^{by}\{a(a-1)y^{a-2}-ay{a-1}\}-(ay^{a-1}-y^a)be^{by}}{e^{2by}}$



The function $f(y) = \frac{y^a}{e^{by}}$ has first derivative:     
$f'(y) = y^{a-1}e^{-by}(a-by)$ 
$f'(y) = \frac{d}{dy}(\frac{y^a}{e^{by}})$        
$f'(y) = y^a(\frac{d}{dy}(e^{-by})) + e^{-by}(\frac{d}{dy}(y^a))$     
$f'(y) = \frac{\frac{d}{dy}(y^a)}{e^{by}} + \frac{\frac{d}{dy}(-(by))}{e^{by}}ya$      
$f'(y) = \frac{\frac{d}{dy}(y^a)}{e^{by}} + \frac{-b\frac{d}{dy}(y)ya}{e^{by}}$       
$f'(y) = \frac{\frac{d}{dy}(y^a)}{e^{by}} + \frac{1by^a}{e^{by}}$      
$f'(y) = \frac{by^a}{e^{by}} + \frac{ay^{a-1}}{e^{by}}$      
